lib/sensor_state.v
@@ -4,14 +4,6 @@ Require Import Bool.
 
 Definition sensor_state := string -> nvalue.
 
-Definition getSens (n:string) (s:sensor_state) : nvalue := s n.
+Definition base_sens (s:string) := default l_fail.
 
-Definition base (s:string) := default l_fail.
-
-Definition contains (s:string) (old:string->nvalue): bool :=
-match (old s) with 
-| default l_fail => false
-| _ => true
-end.
-
-Definition add (s:string) (v:nvalue) (old:string->nvalue): (string->nvalue) :=(fun x => if String.eqb x s then v else (old x)).
+Definition add_sens (s:string) (v:nvalue) (old:string->nvalue): (string->nvalue) :=(fun x => if String.eqb x s then v else (old x)).
